work on fallible specs

case_studies/tests/src/option.rs
@@ -4,12 +4,73 @@ fn maybe_fails() -> Option<i32> {
     Some(2)
 }
 
-// TODO
-#[rr::trust_me]
 #[rr::returns("Some 4")]
 fn get_result() -> Option<i32> {
     let x = maybe_fails()?;
     let y = maybe_fails()?;
 
     Some(x + y)
+}
+
+#[rr::requires("is_Some x")]
+#[rr::exists("y")]
+#[rr::returns("y")]
+fn match_option(x: &Option<i32>) -> i32{
+    if let Some(y) = x {
+        return *y;
+    }
+    else {
+        return 0;
+    }
+}
+
+
+
+#[rr::exists("y")]
+#[rr::returns("y")]
+fn result_get_shr(x: &Result<u32, u32>) -> &u32 {
+    match x {
+        Ok(y) => y,
+        Err(y) => y,
+    }
+}
+
+#[rr::refine_as("Error")]
+enum Error {
+    MyError,
+}
+
+#[rr::returns("Ok 2")]
+fn maybe_fails_2() -> Result<i32, Error> {
+    if let Some(x) = maybe_fails() {
+        Ok(2)
+    }
+    else {
+        Err(Error::MyError)
+    }
+}
+
+
+#[rr::returns("Ok 4")]
+fn get_result_2() -> Result<i32, Error> {
+    let x = maybe_fails_2()?;
+    let y = maybe_fails_2()?;
+
+    Ok(x + y)
+}
+
+#[rr::exists("y")]
+#[rr::ensures("if_Ok y (λ y, y < 10)")]
+#[rr::returns("y")]
+fn maybe_fails_3() -> Result<i32, Error> {
+    Err(Error::MyError)
+}
+
+#[rr::exists("y")]
+#[rr::returns("y")]
+fn get_result_3() -> Result<i32, Error> {
+    let x = maybe_fails_2()?;
+    let y = maybe_fails_3()?;
+
+    Ok(x + y)
 }
