case_studies/tests/output/tests/proofs/proof_option_get_result_3.v
@@ -1,0 +1,47 @@
+From caesium Require Import lang notation.
+From refinedrust Require Import typing shims.
+From refinedrust.examples.tests.generated Require Import generated_code_tests generated_specs_tests generated_template_option_get_result_3.
+
+Set Default Proof Using "Type".
+
+Section proof.
+Context `{RRGS : !refinedrustGS Σ}.
+
+Lemma option_get_result_3_proof (π : thread_id) :
+  option_get_result_3_lemma π.
+Proof.
+  option_get_result_3_prelude.
+
+  rep liRStep; liShow.
+    iApply type_read_ofty_copy.
+    { simpl. apply enum_t_copyable.
+      intros. destruct r; simpl. 
+      - apply _. 
+      - apply struct_t_copy.
+        constructor; last apply _. 
+        apply enum_t_copyable.
+        intros []. apply _.
+    } 
+  repeat liRStep. 
+
+  all: print_remaining_goal.
+  Unshelve. all: sidecond_solver.
+  Unshelve. all: sidecond_hammer.
+  
+
+  (* What is a good way to handle Copyable? *)
+  (* 
+     - Maybe let's just do some manual hackery.
+     - Cleaner: allow attributes to depend on semty, and implement it via trait attrs.
+     TODO.
+
+   *)
+
+
+  (* What is a good way to handle other traits like Send, Sync? *)
+
+
+
+  Unshelve. all: print_remaining_sidecond.
+Admitted.
+End proof.
